doc/tutorial/code/exercises/Ex03b.fst
@@ -17,7 +17,11 @@ module Ex03b
 //fibonacci
 
 
+
 (* Provide several types for the fibonacci function *)
 let rec fibonacci n =
   if n <= 1 then 1 else fibonacci (n - 1) + fibonacci (n - 2)
 
+val fibonacci2 : float -> float
+let rec fibonacci2 n =
+  if n <= 1 then 1 else fibonacci2 (n - 1) + fibonacci2 (n - 2)
