doc/tutorial/code/exercises/Ex04f.fst
@@ -16,7 +16,10 @@
 module Ex04f
 //fold-left
 
-assume val fold_left: f:('b -> 'a -> Tot 'a) -> l:list 'b -> 'a -> Tot 'a
+val fold_left: f:('b -> 'a -> Tot 'a) -> l:list 'b -> 'a -> Tot 'a
+let rec fold_left f l i = match l with
+  | [] -> i
+  | x :: xs -> fold_left f xs (f x i)
 //implement fold_left
 
 val append : list 'a -> list 'a -> Tot (list 'a)
@@ -25,11 +28,32 @@ let rec append l1 l2 = match l1 with
   | hd :: tl -> hd :: append tl l2
 
 val reverse: list 'a -> Tot (list 'a)
-let rec reverse = function 
+let rec reverse = function
   | [] -> []
   | hd::tl -> append (reverse tl) [hd]
 let snoc l h = append l [h]
 
-val fold_left_cons_is_reverse: l:list 'a -> l':list 'a ->
-                             Lemma (fold_left Cons l l' == append (reverse l) l')
-let rec fold_left_cons_is_reverse l l' = admit() //and replace admit() by a proof
+//val list_assoc: l1:list 'a -> l2:list 'a -> l3:list 'a ->
+//                Lemma (append (append l1 l2) l3 == append l1 (append l2 l3))
+//list_assoc l2 l3 l3 =
+
+val list_assoc_elem: l1:list 'a -> b:'a -> l2:list 'a ->
+                Lemma (append l1 (Cons b l2) == append (append l1 [b]) l2)
+let rec list_assoc_elem l1 b l2 = match l1 with
+  | [] -> ()
+  | x :: xs -> list_assoc_elem xs b l2
+
+val fold_left_cons_is_reverse:
+       l:list 'a
+    -> l':list 'a
+    -> Lemma (fold_left Cons l l' == append (reverse l) l')
+let rec fold_left_cons_is_reverse l l' = match l with
+  | [] -> ()
+  | x :: xs -> fold_left_cons_is_reverse xs (Cons x l'); list_assoc_elem (reverse xs) x l'
+
+// fold_left Cons l l'
+// fold_left Cons xs (Cons x l')
+// append (reverse xs) (Cons x l')
+// append (append (reverse xs) [x]) l'
+// append (reverse (x::xs)) l'
+// append (reverse l) l'
