doc/tutorial/code/exercises/Ex04g.fst
@@ -17,4 +17,9 @@ module Ex04g
 //hd-tl
 
 val hd : l:list 'a{Cons? l} -> Tot 'a
+let hd l = match l with
+  | Cons x _ -> x
+
 val tl : l:list 'a{Cons? l} -> Tot (list 'a)
+let tl l = match l with
+  | Cons _ xs -> xs
