doc/tutorial/code/exercises/Ex05b.fst
@@ -16,15 +16,115 @@
 module Ex05b
 //fibonacci-is-ok
 
+
+open FStar.Math.Lemmas
+open FStar.Mul
+open FStar.Squash
+open FStar.SquashProperties
+open FStar.Classical
+
+
+// fib 1 1 0 = 1
+// fib 1 1 1 = fib 1 2 0 = 1
+// fib 1 1 2 = fib 1 2 1 = fib 2 3 0 = 2
+// fib 1 1 3 = fib 1 2 2 = fib 2 3 1 = fib 3 5 0 = 3
+
+// fib a b 1 = fib b (a+b) 0 = b
+// fib a b 2 = fib b (a+b) 1 = fib (a+b) (a+b+b) 0 = a+b
+// fib a b 3 = fib b (a+b) 2 = fib (a+b) (a+b+b) 1 = fib (a+b+b) (a+b+a+b+b) 0 = a+b+b
+// fib a b 4 = fib b (a+b) 3 = fib (a+b) (a+b+b) 2 = fib (a+b+b) (a+b+a+b+b) 1 = fib (a+b+a+b+b) (a+b+b+a+b+a+b+b) 0 = (a+b+a+b+b)
+// fib a b 5 = fib b (a+b) 4 = fib (a+b) (a+b+b) 3 = fib (a+b+b) (a+b+a+b+b) 2 = fib (a+b+a+b+b) (a+b+b+a+b+a+b+b) 1 = .. = (a+b+b+a+b+a+b+b)
+// fib a b 6 = fib b (a+b) 5 = ... = (a+b+b+a+b+a+b+b) + (a+b+a+b+b)
+
+// fib a b n = k1*a + k2*b
+// fib a b (n+1) = fib b (a+b) n = k1*b + k2*(a+b)
+// (k1 = fib (n-2), k2 = fib (n-1))
+
+// ?
+// fib a b 3 = a+b+b
+// fib a (a+b) 3 = b+a+b+a+a = a+b+b + 2*a
+
+// ??
+// fib a b 4 = 2a + 3b
+// fib b (a+b) 4 = 3a + 5b
+// fib a (a+b) 4 = 5a + 3b = fib a b 4 + 3b
+
+// ???
+// fib a b 5 = 3a + 5b
+// fib a (a+b) 5 = 3a + 5b + 5a
+
+// ????
+// fib a b 6 = 5a + 8b
+// fib b (b+a) 6 = 5a + 8b + 5b
+// fib a (a+b) 6 = 8a + 5b + 5a
+
+
+
 val fibonacci : nat -> Tot nat
 let rec fibonacci n =
   if n <= 1 then 1 else fibonacci (n - 1) + fibonacci (n - 2)
 
-val fib : nat -> nat -> n:nat -> Tot nat (decreases n)
+val fib : a:nat -> b:nat -> n:nat -> (Tot (r:nat)) (decreases n)
 let rec fib a b n =
   match n with
   | 0 -> a
   | _ -> fib b (a+b) (n-1)
 
+
+
+
+type fks = tuple2 nat nat
+
+val isfibks : fks -> nat -> nat -> nat -> bool
+let isfibks (k1,k2) a b n =
+    fib a b n = k1 * a + k2 * b
+
+val fibks: a:nat -> b:nat -> n:nat -> Tot (ks:fks{isfibks ks a b n}) (decreases n)
+let rec fibks a b n = match n with
+  | 0 -> (1,0)
+  | 1 -> (0,1)
+  | 2 -> (1,1)
+  | _ -> let (l1,l2) = fibks b (a+b) (n-1) in
+         let (k1,k2) = (l2,l1+l2) in
+         assert (fib a b n = l1 * b + l2 * (a + b));
+         distributivity_add_right l2 a b;
+         assert (fib a b n = l1 * b + l2 * a + l2 * b);
+         assert (fib a b n = l2 * a + (l1 + l2) * b);
+         (k1,k2)
+
+val nextks : fks -> fks
+let nextks (k1,k2) = (k2,k1+k2)
+
+val prevks : ks:fks{snd ks >= fst ks} -> fks
+let prevks (k1,k2) = (k2-k1,k1)
+
+val k2isfact: a:nat -> b:nat -> n:nat{n>=1} -> ks:fks{ks = fibks a b n} ->
+              Lemma (ensures (snd ks = fibonacci (n-1))) (decreases n)
+let rec k2isfact a b n (k1,k2) = match n with
+  | 1 -> assert (k2 = 1)
+  | 2 -> assert (k2 = 1)
+  | _ -> assert (n > 1);
+         k2isfact b (a+b) (n-1) (prevks (k1,k2));
+         assert (k1 = fibonacci (n-2));
+         k2isfact (a+b) (a+b+b) (n-2) (prevks (prevks (k1,k2)));
+         assert (k2-k1 = fibonacci (n-3));
+         assert (k2 = fibonacci (n-1))
+
+val k1isfact: a:nat -> b:nat -> n:nat{n>=2} -> ks:fks{ks = fibks a b n} ->
+              Lemma (ensures (fst ks = fibonacci (n-2))) (decreases n)
+let rec k1isfact a b n (k1,k2) = match n with
+  | 1 -> assert (k1 = 1)
+  | 2 -> assert (k1 = 1)
+  | _ -> k2isfact b (a+b) (n-1) (prevks (k1,k2));
+         k2isfact (a+b) (a+b+b) (n-2) (prevks (prevks (k1,k2)))
+
+val k1plusk2isfact: a:nat -> b:nat -> n:nat{n>=2} -> ks:fks{ks = fibks a b n} ->
+              Lemma (ensures (fst ks + snd ks = fibonacci n))
+let k1plusk2isfact a b n ks = k1isfact a b n ks; k2isfact a b n ks
+
+
 val fib_is_ok : n:nat -> Lemma (fib 1 1 n = fibonacci n)
-let fib_is_ok n = admit() //replace admit() by a proof
+let rec fib_is_ok n = match n with
+  | 0 -> ()
+  | 1 -> ()
+  | _ -> k1plusk2isfact 1 1 n (fibks 1 1 n)
