doc/tutorial/code/exercises/Ex06b.fst
@@ -16,10 +16,58 @@
 module Ex06b
 //quick-sort-poly
 
+open FStar.Option
+open FStar.Classical
+
+//////////////// Comparisons
+
+type total_order (a:eqtype) (f: (a -> a -> Tot bool)) =
+   (forall a1 a2. (f a1 a2 /\ f a2 a1)  ==> a1 = a2)  (* anti-symmetry *)
+ /\ (forall a1 a2 a3. f a1 a2 /\ f a2 a3 ==> f a1 a3)   (* transitivity  *)
+ /\ (forall a1 a2. f a1 a2 \/ f a2 a1)                 (* totality      *)
+
+type cmp (a:eqtype) = f:(a -> a -> Tot bool){total_order a f}
+
+val order_rev: #a:eqtype -> c:(cmp a) -> x:a -> y:a ->
+  Lemma (ensures (not (c x y) ==> c y x))
+let order_rev #a c x y = ()
+
+
+/////////////////////
+
+
 val mem: #t:eqtype -> t -> list t -> Tot bool
 let rec mem #t a l = match l with
   | [] -> false
   | hd::tl -> hd=a || mem a tl
+
+val numocc: #a:eqtype -> a -> list a -> nat
+let rec numocc #a e l = match l with
+  | [] -> 0
+  | x::xs -> (if x = e then 1 else 0) + numocc #a e xs
+
+val numocc_to_mem: #a:eqtype -> e:a -> l:list a -> m:bool{(numocc #a e l > 0) = m /\ mem e l = m}
+let rec numocc_to_mem #a e l = match l with
+  | [] -> false
+  | x::xs -> x = e || numocc_to_mem #a e xs
+
+val numocc_is_mem: #a:eqtype -> e:a -> l:list a ->
+  Lemma (numocc #a e l > 0 = mem e l)
+let numocc_is_mem #a e l =
+  let m = numocc_to_mem #a e l in
+  assert((numocc #a e l > 0) = m /\ mem e l = m)
+
+val numocc_is_mem1: #a:eqtype -> e:a -> l1:list a -> l2:list a ->
+  GTot (u:unit{numocc e l1 = numocc e l2 ==> mem e l1 = mem e l2})
+let rec numocc_is_mem1 #a e l1 l2 = numocc_is_mem #a e l1; numocc_is_mem #a e l2
+
+
+val numocc_is_mem2: #a:eqtype -> l1:list a -> l2:list a ->
+  Lemma (ensures (forall e. numocc e l1 = numocc e l2 ==> mem e l1 = mem e l2))
+  [SMTPat (forall e. numocc e l1 = numocc e l2)]
+let numocc_is_mem2 #a l1 l2 =
+  forall_intro_gtot (fun e -> numocc_is_mem1 e l1 l2)
+
 
 
 val append : list 'a -> list 'a -> Tot (list 'a)
@@ -28,15 +76,16 @@ let rec append l1 l2 = match l1 with
   | hd :: tl -> hd :: append tl l2
 
 
-val append_mem: #t:eqtype 
-	      -> l1:list t
-              -> l2:list t
-              -> Lemma (requires True)
-                       (ensures (forall a. mem a (append l1 l2) = (mem a l1 || mem a l2)))
-                       [SMTPat (append l1 l2)]
-let rec append_mem #t l1 l2 = match l1 with
+val append_numocc:
+       #t:eqtype
+    -> l1:list t
+    -> l2:list t
+    -> Lemma (requires True)
+             (ensures (forall a. numocc a (append l1 l2) = (numocc a l1 + numocc a l2)))
+             [SMTPat (append l1 l2)]
+let rec append_numocc #t l1 l2 = match l1 with
   | [] -> ()
-  | hd::tl -> append_mem tl l2
+  | hd::tl -> append_numocc tl l2
 
 
 val length: list 'a -> Tot nat
@@ -45,11 +94,18 @@ let rec length l = match l with
   | _ :: tl -> 1 + length tl
 
 
-val sorted: list int -> Tot bool
-let rec sorted l = match l with
+val sorted0: list int -> Tot bool
+let rec sorted0 l = match l with
     | [] -> true
     | [x] -> true
-    | x::y::xs -> x <= y && sorted (y::xs)
+    | x::y::xs -> x <= y && sorted0 (y::xs)
+
+
+val sorted: #a:eqtype -> cmp a -> list a -> Tot bool
+let rec sorted #a c l = match l with
+    | [] -> true
+    | [x] -> true
+    | x::y::xs -> c x y && sorted #a c (y::xs)
 
 
 val partition: ('a -> Tot bool) -> list 'a -> Tot (list 'a * list 'a)
@@ -69,34 +125,78 @@ val partition_lemma: #t:eqtype -> f:(t -> Tot bool)
                      + length (snd (partition f l)) = length l
                   /\ (forall x. mem x (fst (partition f l)) ==> f x)
                   /\ (forall x. mem x (snd (partition f l)) ==> not (f x))
-                  /\ (forall x. mem x l = (mem x (fst (partition f l))
-                                        || mem x (snd (partition f l)))))))
+                  /\ (forall x. numocc x l =
+                                numocc x (fst (partition f l)) +
+                                numocc x (snd (partition f l))))))
             [SMTPat (partition f l)]
 let rec partition_lemma #t f l = match l with
     | [] -> ()
     | hd::tl -> partition_lemma f tl
 
 
-val sorted_concat_lemma: l1:list int{sorted l1}
-                      -> l2:list int{sorted l2}
-                      -> pivot:int
-                      -> Lemma (requires ((forall y. mem y l1 ==> not (pivot <= y))
-                                       /\ (forall y. mem y l2 ==> pivot <= y)))
-                               (ensures (sorted (append l1 (pivot::l2))))
-                               [SMTPat (sorted (append l1 (pivot::l2)))]
-let rec sorted_concat_lemma l1 l2 pivot = match l1 with
+val sorted_concat_lemma0:
+       l1:list int{sorted0 l1}
+    -> l2:list int{sorted0 l2}
+    -> pivot:int
+    -> Lemma (requires ((forall y. mem y l1 ==> not (pivot <= y))
+                     /\ (forall y. mem y l2 ==> pivot <= y)))
+             (ensures (sorted0 (append l1 (pivot::l2))))
+             [SMTPat (sorted0 (append l1 (pivot::l2)))]
+let rec sorted_concat_lemma0 l1 l2 pivot = match l1 with
     | [] -> ()
-    | hd::tl -> sorted_concat_lemma tl l2 pivot
+    | hd::hd2::tl -> sorted_concat_lemma0 tl l2 pivot; assert (hd <= hd2)
+    | hd::tl -> sorted_concat_lemma0 tl l2 pivot; assert (hd <= pivot)
 
+val sorted_concat_lemma:
+       #a:eqtype
+    -> c:(cmp a)
+    -> l1:list a{sorted c l1}
+    -> l2:list a{sorted c l2}
+    -> pivot:a
+    -> Lemma (requires ((forall y. mem y l1 ==> not (c pivot y))
+                     /\ (forall y. mem y l2 ==> c pivot y)))
+             (ensures (sorted c (append l1 (pivot::l2))))
+             [SMTPat (sorted c (append l1 (pivot::l2)))]
+let rec sorted_concat_lemma #a c l1 l2 pivot = match l1 with
+    | [] -> ()
+    | [hd] -> sorted_concat_lemma #a c [] l2 pivot;
+              order_rev #a c pivot hd
+    | hd::hd'::tl' -> sorted_concat_lemma #a c (hd'::tl') l2 pivot
 
-val sort: l:list int -> Tot (m:list int{sorted m /\ (forall i. mem i l = mem i m)})
-                            (decreases (length l))
-let rec sort l = match l with
+#set-options "--z3rlimit 90 --initial_fuel 5 --max_fuel 5 --initial_ifuel 2 --max_ifuel 2"
+
+val sort: #a:eqtype -> c:(cmp a) -> l:list a ->
+          Tot ( m:list a{ sorted c m /\
+                          (forall i. numocc i l = numocc i m) })
+              (decreases (length l))
+let rec sort #a c l = match l with
   | [] -> []
   | pivot::tl ->
-    let hi, lo = partition (fun j -> pivot <= j) tl in
-    let m = append (sort lo) (pivot::sort hi) in
-    assert (forall i. mem i (pivot :: sort hi) = mem i (append [pivot] (sort hi)));
-    m
+    let hi, lo = partition (fun j -> c pivot j) tl in
+    let los = sort #a c lo in
+    let his = sort #a c hi in
+    let m = append los (pivot::his) in
 
-    
+    numocc_is_mem2 los lo;
+    numocc_is_mem2 his hi;
+    assert(forall i. mem i los = mem i lo);
+    assert(forall i. mem i his = mem i hi);
+
+    sorted_concat_lemma #a c los his pivot;
+    assert (sorted c m);
+
+
+    // Numocc
+    assert (forall i. numocc i los = numocc i lo);
+    assert (forall i. numocc i his = numocc i hi);
+    assert (forall i. numocc i l = numocc i lo + numocc i [pivot] + numocc i hi);
+    assert (forall i. numocc i m = numocc i los + numocc i (pivot::his));
+    assert (forall i. numocc i m = numocc i lo + numocc i [pivot] + numocc i hi);
+    assert (forall i. numocc i m = numocc i l);
+    assert (forall i. numocc i l = numocc i m);
+
+
+    assert (sorted c m /\ (forall i. numocc i l = numocc i m));
+
+
+    m
