doc/tutorial/code/exercises/Ex10b.fst
@@ -21,12 +21,13 @@ open FStar.Ref
 noeq type point =
   | Point : x:ref int -> y:ref int{addr_of y <> addr_of x} -> point
 
+
 val new_point: x:int -> y:int -> ST point
   (requires (fun h -> True))
   (ensures (fun h0 p h1 ->
                 modifies Set.empty h0 h1
                 /\ fresh (Point?.x p) h0 h1
-		/\ fresh (Point?.y p) h0 h1
+                /\ fresh (Point?.y p) h0 h1
                 /\ Heap.sel h1 (Point?.x p) = x
                 /\ Heap.sel h1 (Point?.y p) = y))
 let new_point x y =
@@ -34,24 +35,29 @@ let new_point x y =
   let y = alloc y in
   Point x y
 
-let shift_x p =
-  Point?.x p := !(Point?.x p) + 1
+val shift: p:point -> ST unit
+  (requires (fun _ -> True))
+  (ensures (fun h0 _ h1 -> modifies (Point?.x p ^+^ Point?.y p) h0 h1))
+let shift p =
+  Point?.x p := !(Point?.x p) + 1;
+  Point?.y p := !(Point?.y p) + 5
 
 // BEGIN: ShiftXP1Spec
-val shift_x_p1: p1:point
+val shift_p1: p1:point
            -> p2:point{   addr_of (Point?.x p2) <> addr_of (Point?.x p1)
+                       /\ addr_of (Point?.y p2) <> addr_of (Point?.y p1)
+                       /\ addr_of (Point?.x p2) <> addr_of (Point?.y p1)
                        /\ addr_of (Point?.y p2) <> addr_of (Point?.x p1) }
            -> ST unit
     (requires (fun h -> Heap.contains h (Point?.x p2)
                     /\  Heap.contains h (Point?.y p2)))
-    (ensures (fun h0 _ h1 -> modifies (only (Point?.x p1)) h0 h1))
+    (ensures (fun h0 _ h1 -> modifies (Point?.x p1 ^+^ Point?.y p1) h0 h1))
 // END: ShiftXP1Spec
 
-let shift_x_p1 p1 p2 =
+let shift_p1 p1 p2 =
     let p2_0 = !(Point?.x p2), !(Point?.y p2)  in //p2 is initially p2_0
-    shift_x p1;
+    shift p1;
     let p2_1 = !(Point?.x p2), !(Point?.y p2) in
-    admit(); //fix the precondition and remove the admit
     assert (p2_0 = p2_1)                         //p2 is unchanged
 
 
@@ -63,4 +69,4 @@ let test () =
   let p2 = new_point 0 1 in
   recall (Point?.x p2);
   recall (Point?.y p2);
-  shift_x_p1 p1 p2
+  shift_p1 p1 p2
