doc/tutorial/code/exercises/Ex04b.fst
@@ -27,8 +27,10 @@ let rec append l1 l2 = match l1 with
   | hd :: tl -> hd :: append tl l2
 
 (* Prove this lemma *)
-val append_len: l1:list 'a -> l2:list 'a 
+val append_len: l1:list 'a -> l2:list 'a
          -> Lemma (requires True)
                   (ensures (length (append l1 l2) = length l1 + length l2))
-let rec append_len l1 l2 = admit() //remove admit() and write proof
-
+let rec append_len l1 l2 =
+  match l1 with
+  | [] -> ()
+  | x :: xs -> append_len xs l2
