doc/tutorial/code/exercises/Ex12.MAC.fst
@@ -27,10 +27,10 @@ module SHA1 = Ex12.SHA1
 
 (* ---- specification *)
 
-(* We make the MAC.key abstract so that it cannot be accessed by 
+(* We make the MAC.key abstract so that it cannot be accessed by
    the adversary *)
 
-abstract type key=SHA1.key 
+abstract type key=SHA1.key
 
 (* we attach an authenticated properties to each key,
    used as a pre-condition for MACing and
@@ -57,11 +57,11 @@ let log:log_t = ST.alloc #(list entry) []
 
 // BEGIN: MacSpec
 val keygen: p:(text -> Type) -> ML (pkey p)
-val mac:    k:key -> t:text{key_prop k t} -> ST tag 
-  (requires (fun h -> True)) 
+val mac:    k:key -> t:text{key_prop k t} -> ST tag
+  (requires (fun h -> True))
   (ensures (fun h x h' -> Heap.modifies (Heap.only log) h h'))
-val verify: k:key -> t:text -> tag -> ST (b:bool{b ==> key_prop k t}) 
-  (requires (fun h -> True)) 
+val verify: k:key -> t:text -> tag -> ST (b:bool{b ==> key_prop k t})
+  (requires (fun h -> True))
   (ensures (fun h x h' -> Heap.modifies Set.empty h h'))
 // END: MacSpec
 
