ulib/FStar.Monotonic.Heap.fsti
@@ -100,28 +100,28 @@ let equal_dom (h1:heap) (h2:heap) :GTot Type0 =
 val lemma_ref_unused_iff_addr_unused (#a:Type0) (#rel:preorder a) (h:heap) (r:mref a rel)
   :Lemma (requires True)
          (ensures  (r `unused_in` h <==> addr_of r `addr_unused_in` h))
-	 [SMTPatOr [[SMTPat (r `unused_in` h)]; [SMTPat (addr_of r `addr_unused_in` h)]]]
+     [SMTPatOr [[SMTPat (r `unused_in` h)]; [SMTPat (addr_of r `addr_unused_in` h)]]]
 
 val lemma_contains_implies_used (#a:Type0) (#rel:preorder a) (h:heap) (r:mref a rel)
   :Lemma (requires (h `contains` r))
          (ensures  (~ (r `unused_in` h)))
-	 [SMTPatOr [[SMTPat (h `contains` r)]; [SMTPat (r `unused_in` h)]]]
+     [SMTPatOr [[SMTPat (h `contains` r)]; [SMTPat (r `unused_in` h)]]]
 
 val lemma_distinct_addrs_distinct_types
   (#a:Type0) (#b:Type0) (#rel1:preorder a) (#rel2:preorder b) (h:heap) (r1:mref a rel1) (r2:mref b rel2)
   :Lemma (requires (a =!= b /\ h `contains` r1 /\ h `contains` r2))
          (ensures  (addr_of r1 <> addr_of r2))
-	 [SMTPat (h `contains` r1); SMTPat (h `contains` r2)]
+     [SMTPat (h `contains` r1); SMTPat (h `contains` r2)]
 
 val lemma_distinct_addrs_distinct_preorders (u:unit)
   :Lemma (forall (a:Type0) (rel1 rel2:preorder a) (r1:mref a rel1) (r2:mref a rel2) (h:heap).
             {:pattern (h `contains` r1); (h `contains` r2)}
-	    (h `contains` r1 /\ h `contains` r2 /\ rel1 =!= rel2) ==> addr_of r1 <> addr_of r2)
+        (h `contains` r1 /\ h `contains` r2 /\ rel1 =!= rel2) ==> addr_of r1 <> addr_of r2)
 
 val lemma_distinct_addrs_distinct_mm (u:unit)
   :Lemma (forall (a b:Type0) (rel1:preorder a) (rel2:preorder b) (r1:mref a rel1) (r2:mref b rel2) (h:heap).
             {:pattern (h `contains` r1); (h `contains` r2)}
-	    (h `contains` r1 /\ h `contains` r2 /\ is_mm r1 =!= is_mm r2) ==> addr_of r1 <> addr_of r2)
+        (h `contains` r1 /\ h `contains` r2 /\ is_mm r1 =!= is_mm r2) ==> addr_of r1 <> addr_of r2)
 
 (*
  * AR: this is a bit surprising. i had to add ~ (r1 === r2) postcondition to make the lemma
@@ -138,32 +138,32 @@ val lemma_alloc (#a:Type0) (rel:preorder a) (h0:heap) (x:a) (mm:bool)
   :Lemma (requires True)
          (ensures  (let r, h1 = alloc rel h0 x mm in
                     fresh r h0 h1 /\ h1 == upd h0 r x /\ is_mm r = mm /\ addr_of r == next_addr h0))
-	 [SMTPat (alloc rel h0 x mm)]
+     [SMTPat (alloc rel h0 x mm)]
 
 val lemma_free_mm_sel
   (#a:Type0) (#b:Type0) (#rel1:preorder a) (#rel2:preorder b) (h0:heap)
   (r1:mref a rel1{h0 `contains` r1 /\ is_mm r1}) (r2:mref b rel2)
   :Lemma (requires True)
          (ensures  (addr_of r2 <> addr_of r1 ==> sel h0 r2 == sel (free_mm h0 r1) r2))
-	 [SMTPat (sel (free_mm h0 r1) r2)]
+     [SMTPat (sel (free_mm h0 r1) r2)]
 
 val lemma_free_mm_contains
   (#a:Type0) (#b:Type0) (#rel1:preorder a) (#rel2:preorder b) (h0:heap)
   (r1:mref a rel1{h0 `contains` r1 /\ is_mm r1}) (r2:mref b rel2)
   :Lemma (requires True)
          (ensures  (let h1 = free_mm h0 r1 in
-	            (addr_of r2 <> addr_of r1 /\ h0 `contains` r2) <==> h1 `contains` r2))
-	 [SMTPat ((free_mm h0 r1) `contains` r2)]
+                (addr_of r2 <> addr_of r1 /\ h0 `contains` r2) <==> h1 `contains` r2))
+     [SMTPat ((free_mm h0 r1) `contains` r2)]
 
 val lemma_free_mm_unused
   (#a:Type0) (#b:Type0) (#rel1:preorder a) (#rel2:preorder b) (h0:heap)
   (r1:mref a rel1{h0 `contains` r1 /\ is_mm r1}) (r2:mref b rel2)
   :Lemma (requires True)
          (ensures  (let h1 = free_mm h0 r1 in
-	            ((addr_of r1 = addr_of r2 ==> r2 `unused_in` h1)      /\
-		     (r2 `unused_in` h0       ==> r2 `unused_in` h1)      /\
-		     (r2 `unused_in` h1       ==> (r2 `unused_in` h0 \/ addr_of r2 = addr_of r1)))))
-	 [SMTPat (r2 `unused_in` (free_mm h0 r1))]
+                ((addr_of r1 = addr_of r2 ==> r2 `unused_in` h1)      /\
+             (r2 `unused_in` h0       ==> r2 `unused_in` h1)      /\
+             (r2 `unused_in` h1       ==> (r2 `unused_in` h0 \/ addr_of r2 = addr_of r1)))))
+     [SMTPat (r2 `unused_in` (free_mm h0 r1))]
 
 val lemma_free_addr_unused_in
   (#a: Type) (#rel: preorder a) (h: heap) (r: mref a rel { h `contains` r /\ is_mm r } )
@@ -180,7 +180,7 @@ val lemma_sel_same_addr (#a:Type0) (#rel:preorder a) (h:heap) (r1:mref a rel) (r
   :Lemma (requires (h `contains` r1 /\ addr_of r1 = addr_of r2 /\ is_mm r1 == is_mm r2))
          (ensures  (h `contains` r2 /\ sel h r1 == sel h r2))
          [SMTPatOr [
-	   [SMTPat (sel h r1); SMTPat (sel h r2)];
+       [SMTPat (sel h r1); SMTPat (sel h r2)];
            [SMTPat (h `contains` r1); SMTPat (h `contains` r2)];
          ]]
 
@@ -195,7 +195,7 @@ val lemma_sel_upd1 (#a:Type0) (#rel:preorder a) (h:heap) (r1:mref a rel) (x:a) (
 val lemma_sel_upd2 (#a:Type0) (#b:Type0) (#rel1:preorder a) (#rel2:preorder b) (h:heap) (r1:mref a rel1) (r2:mref b rel2) (x:b)
   :Lemma (requires (addr_of r1 <> addr_of r2))
          (ensures  (sel (upd h r2 x) r1 == sel h r1))
-	 [SMTPat (sel (upd h r2 x) r1)]
+     [SMTPat (sel (upd h r2 x) r1)]
 
 val lemma_mref_injectivity
   :(u:unit{forall (a:Type0) (b:Type0) (rel1:preorder a) (rel2:preorder b) (r1:mref a rel1) (r2:mref b rel2). a =!= b ==> ~ (eq3 r1 r2)})
@@ -203,39 +203,39 @@ val lemma_mref_injectivity
 val lemma_in_dom_emp (#a:Type0) (#rel:preorder a) (r:mref a rel)
   :Lemma (requires True)
          (ensures  (r `unused_in` emp))
-	 [SMTPat (r `unused_in` emp)]
+     [SMTPat (r `unused_in` emp)]
 
 val lemma_upd_contains (#a:Type0) (#rel:preorder a) (h:heap) (r:mref a rel) (x:a)
   :Lemma (requires True)
          (ensures  ((upd h r x) `contains` r))
-	 [SMTPat ((upd h r x) `contains` r)]
+     [SMTPat ((upd h r x) `contains` r)]
 
 val lemma_well_typed_upd_contains
   (#a:Type0) (#b:Type0) (#rel1:preorder a) (#rel2:preorder b) (h:heap) (r1:mref a rel1) (x:a) (r2:mref b rel2)
   :Lemma (requires (h `contains` r1))
          (ensures  (let h1 = upd h r1 x in
-	            h1 `contains` r2 <==> h `contains` r2))
-	 [SMTPat ((upd h r1 x) `contains` r2)]
+                h1 `contains` r2 <==> h `contains` r2))
+     [SMTPat ((upd h r1 x) `contains` r2)]
 
 val lemma_unused_upd_contains
   (#a:Type0) (#b:Type0) (#rel1:preorder a) (#rel2:preorder b) (h:heap) (r1:mref a rel1) (x:a) (r2:mref b rel2)
   :Lemma (requires (r1 `unused_in` h))
          (ensures  (let h1 = upd h r1 x in
-	            (h `contains` r2  ==> h1 `contains` r2) /\
-		    (h1 `contains` r2 ==> (h `contains` r2 \/ addr_of r2 = addr_of r1))))
-	 [SMTPat ((upd h r1 x) `contains` r2)]
+                (h `contains` r2  ==> h1 `contains` r2) /\
+            (h1 `contains` r2 ==> (h `contains` r2 \/ addr_of r2 = addr_of r1))))
+     [SMTPat ((upd h r1 x) `contains` r2)]
 
 val lemma_upd_contains_different_addr
   (#a:Type0) (#b:Type0) (#rel1:preorder a) (#rel2:preorder b) (h:heap) (r1:mref a rel1) (x:a) (r2:mref b rel2)
   :Lemma (requires (h `contains` r2 /\ addr_of r1 <> addr_of r2))
          (ensures  ((upd h r1 x) `contains` r2))
-	 [SMTPat ((upd h r1 x) `contains` r2)]
+     [SMTPat ((upd h r1 x) `contains` r2)]
 
 val lemma_upd_unused
   (#a:Type0) (#b:Type0) (#rel1:preorder a) (#rel2:preorder b) (h:heap) (r1:mref a rel1) (x:a) (r2:mref b rel2)
   :Lemma (requires True)
          (ensures  ((addr_of r1 <> addr_of r2 /\ r2 `unused_in` h) <==> r2 `unused_in` (upd h r1 x)))
-	 [SMTPat (r2 `unused_in` (upd h r1 x))]
+     [SMTPat (r2 `unused_in` (upd h r1 x))]
 
 val lemma_contains_upd_modifies (#a:Type0) (#rel:preorder a) (h:heap) (r:mref a rel) (x:a)
   :Lemma (requires (h `contains` r))
@@ -261,7 +261,7 @@ val lemma_modifies_and_equal_dom_sel_diff_addr
   (#a:Type0)(#rel:preorder a) (s:set nat) (h0:heap) (h1:heap) (r:mref a rel)
   :Lemma (requires (modifies s h0 h1 /\ equal_dom h0 h1 /\ (~ (S.mem (addr_of r) s))))
          (ensures  (sel h0 r == sel h1 r))
-	 [SMTPat (modifies s h0 h1); SMTPat (equal_dom h0 h1); SMTPat (sel h1 r)]
+     [SMTPat (modifies s h0 h1); SMTPat (equal_dom h0 h1); SMTPat (sel h1 r)]
 
 val lemma_heap_equality_upd_same_addr (#a: Type0) (#rel: preorder a) (h: heap) (r1 r2: mref a rel) (x: a)
   :Lemma (requires ((h `contains` r1 \/ h `contains` r2) /\ addr_of r1 = addr_of r2 /\ is_mm r1 == is_mm r2))
